Use Joe's sets instead of lists

theories/Environment.v
@@ -5,6 +5,7 @@ From LambdaST Require Import
   Hole
   Ident
   Prefix
+  Sets
   Terms
   Types.
 From Hammer Require Import
@@ -13,20 +14,20 @@ From Hammer Require Import
 Definition env : Set := ident -> option prefix.
 Hint Unfold env : core.
 
-Definition subst : ident -> prefix -> env -> env := fun id p n x => if eq_id id x then Some p else n x.
-Arguments subst p n x/.
-Hint Unfold subst : core.
+Definition env_subst : ident -> prefix -> env -> env := fun id p n x => if eq_id id x then Some p else n x.
+Arguments env_subst p n x/.
+Hint Unfold env_subst : core.
 
-Definition union : env -> env -> env := fun n n' x => match n' x with None => n x | Some y => Some y end.
-Arguments union n n' x/.
-Hint Unfold union : core.
+Definition env_union : env -> env -> env := fun n n' x => match n' x with None => n x | Some y => Some y end.
+Arguments env_union n n' x/.
+Hint Unfold env_union : core.
 
 (* Theorem B.10, part I *)
 Theorem maps_to_unique_literal : forall p x (n : env),
   n x = Some p ->
   ~exists q, p <> q /\ n x = Some q.
 Proof.
-  intros p x n Hp [q [Hpq Hq]]. cbn in *. rewrite Hp in Hq. sinvert Hq. apply Hpq. reflexivity.
+  intros p x n Hp [q [Hpq Hq]]. rewrite Hp in Hq. sinvert Hq. apply Hpq. reflexivity.
 Qed.
 Hint Resolve maps_to_unique_literal : core.
 
@@ -38,26 +39,29 @@ Proof. intros p1 p2 x n H1 H2. cbn in *. rewrite H1 in H2. sinvert H2. reflexivi
 Hint Resolve maps_to_unique : core.
 
 (* Generalization of `emptyOn` and `maximalOn` from the paper *)
-Definition prop_on_item : (prefix -> Prop) -> env -> ident -> Prop :=
+Definition PropOnItem : (prefix -> Prop) -> env -> ident -> Prop :=
   fun P n x => exists p, n x = Some p /\ P p.
-Arguments prop_on_item P n x/.
-Hint Unfold prop_on_item : core.
+Arguments PropOnItem P n x/.
+Hint Unfold PropOnItem : core.
 
-Definition PropOn : (prefix -> Prop) -> context -> env -> Prop := fun P s n => Forall (prop_on_item P n) (vars_in s).
-Arguments PropOn/ P s n.
+Definition PropOn (P : prefix -> Prop) (ctx : context) (n : env) : Prop :=
+  SetProp (PropOnItem P n) (vars_in ctx).
+Arguments PropOn/ P ctx n.
 Hint Unfold PropOn : core.
 
-Definition EmptyOn := PropOn Empty.
-Arguments EmptyOn/ s n.
+Definition EmptyOn := PropOn EmptyPfx.
+Arguments EmptyOn/ ctx n.
 Hint Unfold EmptyOn : core.
 
-Definition MaximalOn := PropOn Maximal.
-Arguments MaximalOn/ s n.
+Definition MaximalOn := PropOn MaximalPfx.
+Arguments MaximalOn/ ctx n.
 Hint Unfold MaximalOn : core.
 
 (* TODO: empty/maximal on (free variables in) terms *)
 
-Definition Agree n n' D D' : Prop := (MaximalOn D n <-> MaximalOn D' n') /\ (EmptyOn D n <-> EmptyOn D' n').
+Definition Agree (n n' : env) (D D' : context) : Prop :=
+  (MaximalOn D n <-> MaximalOn D' n') /\
+  (EmptyOn D n <-> EmptyOn D' n').
 Arguments Agree/ n n' D D'.
 Hint Unfold Agree : core.
 
@@ -99,39 +103,59 @@ Proof. intros. assert (A := maps_to_hole _ _ _ H). sinvert A. eexists. split; ea
 Hint Resolve maps_to_has_type : core.
 
 Lemma prop_on_item_weakening : forall P n n' vs,
-  prop_on_item P n' vs ->
-  prop_on_item P (union n n') vs.
+  PropOnItem P n' vs ->
+  PropOnItem P (env_union n n') vs.
 Proof. intros P n n' vs [p [Hn' Hp]]. exists p. split; [| assumption]. cbn. rewrite Hn'. reflexivity. Qed.
 Hint Resolve prop_on_item_weakening : core.
 
+Lemma prop_on_weakening : forall P nr nl ctx,
+  PropOn P ctx nr ->
+  PropOn P ctx (env_union nl nr).
+Proof. sfirstorder use:prop_on_item_weakening. Qed.
+Hint Resolve prop_on_weakening : core.
+
+Lemma empty_on_weakening : forall nr nl ctx,
+  EmptyOn ctx nr ->
+  EmptyOn ctx (env_union nl nr).
+Proof. apply prop_on_weakening. Qed.
+Hint Resolve empty_on_weakening : core.
+
+Lemma maximal_on_weakening : forall nr nl ctx,
+  MaximalOn ctx nr ->
+  MaximalOn ctx (env_union nl nr).
+Proof. apply prop_on_weakening. Qed.
+Hint Resolve maximal_on_weakening : core.
+
 Lemma env_typed_weakening : forall n n' G,
   EnvTyped n' G ->
-  EnvTyped (union n n') G.
+  EnvTyped (env_union n n') G.
 Proof.
   intros n n' G H. generalize dependent n.
   induction H; intros; econstructor;
   try apply IHEnvTyped1; try apply IHEnvTyped2;
   [cbn; rewrite H; reflexivity | assumption |].
-  destruct H1; [left | right]; (eapply Forall_impl in H1; [apply H1 | apply prop_on_item_weakening]).
+  destruct H1; [left | right]; apply prop_on_weakening; assumption.
 Qed.
 Hint Resolve env_typed_weakening : core.
 
 Definition NoConflict (n n' : env) := forall x p,
-  n x = Some p -> (n' x = None \/ n' x = Some p).
+  n x = Some p ->
+  forall p',
+  n' x = Some p' ->
+  p = p'.
 Arguments NoConflict/ n n'.
 Hint Unfold NoConflict : core.
 
 Lemma env_typed_weakening_alt : forall n n' G,
   NoConflict n n' ->
   EnvTyped n G ->
-  EnvTyped (union n n') G.
+  EnvTyped (env_union n n') G.
 Proof.
   intros n n' G Hm Ht. generalize dependent n'.
   induction Ht; intros; cbn in *; econstructor; try apply IHHt1; try apply IHHt2; try eassumption.
-  - cbn. specialize (Hm _ _ H) as [Hm | Hm]; rewrite Hm; [assumption | reflexivity].
-  - destruct H; [left | right]; (eapply Forall_impl; [| eassumption]); intros; cbn in *;
-    destruct H0 as [p [Hpn Hp]]; eexists; (split; [| eassumption]);
-    (specialize (Hm _ _ Hpn) as [Hm | Hm]; rewrite Hm; [assumption | reflexivity]).
+  - cbn. specialize (Hm _ _ H). destruct (n' x) as [p' |] eqn:E. 2: { assumption. }
+    f_equal. symmetry. apply Hm. reflexivity.
+  - destruct H; hauto q: on db: core. (* TODO: speed this up *)
 Qed.
 Hint Resolve env_typed_weakening_alt : core.
 
@@ -141,7 +165,7 @@ Lemma agree_union : forall P n n' D D' lhs lhs' lhs'',
   FillWith D  lhs lhs'  ->
   FillWith D' lhs lhs'' ->
   PropOn P lhs' n ->
-  PropOn P lhs'' (union n n').
+  PropOn P lhs'' (env_union n n').
 Proof.
   intros P n n' D D' lhs lhs' lhs'' Hn Hp Hf Hf' H. generalize dependent P. generalize dependent n. generalize dependent n'.
   generalize dependent D'. generalize dependent lhs''. induction Hf; intros; sinvert Hf'; cbn in *; [
